examples/lpr_checker/array/README.md
@@ -3,8 +3,8 @@ Improving the LRAT checker with arrays (manually)
 [compilation](compilation):
 An LRAT checker built on CakeML with arrays
 
-[lrat_arrayProgScript.sml](lrat_arrayProgScript.sml):
-This refines lrat_list to use arrays
+[lpr_arrayProgScript.sml](lpr_arrayProgScript.sml):
+This refines lpr_list to use arrays
 
-[lrat_listScript.sml](lrat_listScript.sml):
+[lpr_listScript.sml](lpr_listScript.sml):
 This refines the LPR checker to a fixed-size, list-based implementation
