examples/lpr_checker/array/compilation/README.md
@@ -1,7 +1,7 @@
 An LRAT checker built on CakeML with arrays
 
-[lrat_arrayCompileScript.sml](lrat_arrayCompileScript.sml):
-Compiles the lrat example by evaluation inside the logic of HOL
+[lpr_arrayCompileScript.sml](lpr_arrayCompileScript.sml):
+Compiles the lpr example by evaluation inside the logic of HOL
 
 [proofs](proofs):
 Prove end-to-end correctness theorem for LRAT checker with arrays
